Fix core simplification theory

src/tools/symbexec/bir_symb_simpScript.sml
@@ -7,9 +7,17 @@ open symb_auxTheory;
 
 open symb_rulesTheory;
 
+open bir_symbTheory;
+open bir_symb_sound_coreTheory;
+
 open arithmeticTheory;
 open pred_setTheory;
 
+open symb_typesLib;
+
+(*
+val birs_state_ss = rewrites (type_rws ``:birs_state_t``);
+*)
 
 val _ = new_theory "bir_symb_simp";
 
@@ -34,7 +42,7 @@ val symb_simplification_thm = store_thm(
   (symb_simplification sr sys symbexp symbexp') ==>
   (symb_simplification_e sr (symb_symbst_pcond sys) symbexp symbexp')
 ``,
-  METIS_TAC [symb_simplification_def, symb_simplification_e_def, symb_interpr_symbpcond_def]
+  REWRITE_TAC [symb_simplification_def, symb_simplification_e_def, symb_interpr_symbpcond_def]
 );
 
 val symb_exp_imp_def = Define `
@@ -59,33 +67,112 @@ val symb_simplification_IMP_thm = store_thm(
   (symb_simplification_e sr pcond' symbexp symbexp') ==>
   (symb_simplification_e sr pcond  symbexp symbexp')
 ``,
-  cheat
+  REWRITE_TAC [symb_exp_imp_def, symb_simplification_e_def] >>
+  REPEAT STRIP_TAC >>
+
+  `symb_interpr_for_symbs (sr.sr_symbols_f pcond) H` by (
+    FULL_SIMP_TAC std_ss [symb_interpr_for_symbs_def, UNION_SUBSET]
+  ) >>
+
+  `symb_interpr_for_symbs
+          (sr.sr_symbols_f pcond' UNION sr.sr_symbols_f symbexp UNION
+           sr.sr_symbols_f symbexp') H` by (
+    FULL_SIMP_TAC std_ss [symb_interpr_for_symbs_def, UNION_SUBSET] >>
+    METIS_TAC [SUBSET_TRANS]
+  ) >>
+
+  METIS_TAC []
 );
+
+
+val birs_simplification_e_def = Define `
+    birs_simplification_e pcond symbexp symbexp' =
+    (!H.
+       (birs_interpr_welltyped H) ==>
+       (symb_interpr_for_symbs
+            ((bir_vars_of_exp pcond) UNION
+             (bir_vars_of_exp symbexp) UNION
+             (bir_vars_of_exp symbexp')) H) ==>
+
+       (birs_interpret_fun H pcond = SOME bir_val_true) ==>
+       (birs_interpret_fun H symbexp = birs_interpret_fun H symbexp')
+    )
+`;
+
+val birs_simplification_e_thm = store_thm(
+   "birs_simplification_e_thm", ``
+!prog.
+!pcond symbexp symbexp'.
+  (symb_simplification_e (bir_symb_rec_sbir prog) pcond symbexp symbexp') <=>
+  (birs_simplification_e pcond symbexp symbexp')
+``,
+  REWRITE_TAC [symb_simplification_e_def, birs_simplification_e_def] >>
+  REWRITE_TAC [birs_interpr_welltyped_EQ_thm] >>
+  SIMP_TAC (std_ss++symb_TYPES_ss) [bir_symb_rec_sbir_def]
+);
+
+val birs_exp_imp_def = Define `
+    birs_exp_imp pcond pcond' =
+    ((bir_vars_of_exp pcond' SUBSET bir_vars_of_exp pcond) /\
+     (!H.
+       (birs_interpr_welltyped H) ==>
+       (symb_interpr_for_symbs
+            (bir_vars_of_exp pcond) H) ==>
+
+       (birs_interpret_fun H pcond  = SOME bir_val_true) ==>
+       (birs_interpret_fun H pcond' = SOME bir_val_true)
+     )
+    )
+`;
+
+val birs_exp_imp_thm = store_thm(
+   "birs_exp_imp_thm", ``
+!prog.
+!pcond pcond'.
+  (symb_exp_imp (bir_symb_rec_sbir prog) pcond pcond') <=>
+  (birs_exp_imp pcond pcond')
+``,
+  REWRITE_TAC [symb_exp_imp_def, birs_exp_imp_def] >>
+  REWRITE_TAC [birs_interpr_welltyped_EQ_thm] >>
+  SIMP_TAC (std_ss++symb_TYPES_ss) [bir_symb_rec_sbir_def]
+);
+
+val birs_simplification_IMP_thm = store_thm(
+   "birs_simplification_IMP_thm", ``
+!pcond pcond' symbexp symbexp'.
+  (birs_exp_imp pcond pcond') ==>
+  (birs_simplification_e pcond' symbexp symbexp') ==>
+  (birs_simplification_e pcond  symbexp symbexp')
+``,
+  METIS_TAC [symb_simplification_IMP_thm, birs_simplification_e_thm, birs_exp_imp_thm]
+);
+
+
+
+
+
 
 val symb_simplification_UnsignedCast_thm = store_thm(
    "symb_simplification_UnsignedCast_thm", ``
-!sr.
 !pcond symbexp symbexp' sz.
-  (symb_simplification_e sr pcond symbexp symbexp') ==>
-  (symb_simplification_e sr pcond (BExp_Cast BIExp_UnsignedCast symbexp sz) (BExp_Cast BIExp_UnsignedCast symbexp' sz))
+  (birs_simplification_e pcond symbexp symbexp') ==>
+  (birs_simplification_e pcond (BExp_Cast BIExp_UnsignedCast symbexp sz) (BExp_Cast BIExp_UnsignedCast symbexp' sz))
 ``,
   cheat
 );
 
 val symb_simplification_IfThenElse_T_thm = store_thm(
    "symb_simplification_IfThenElse_T_thm", ``
-!sr.
 !pcond ec et ef.
-  (symb_simplification_e sr ec (BExp_IfThenElse ec et ef) et)
+  (birs_simplification_e ec (BExp_IfThenElse ec et ef) et)
 ``,
   cheat
 );
 
 val symb_simplification_IfThenElse_F_thm = store_thm(
    "symb_simplification_IfThenElse_F_thm", ``
-!sr.
 !pcond ec et ef.
-  (symb_simplification_e sr (BExp_UnaryExp BIExp_Not ec) (BExp_IfThenElse ec et ef) ef)
+  (birs_simplification_e (BExp_UnaryExp BIExp_Not ec) (BExp_IfThenElse ec et ef) ef)
 ``,
   cheat
 );
@@ -93,11 +180,10 @@ val symb_simplification_IfThenElse_F_thm = store_thm(
 (* TODO: need to typecheck the whole expression, also in the next theorem *)
 val symb_simplification_Mem_Match_thm = store_thm(
    "symb_simplification_Mem_Match_thm", ``
-!sr.
 !be_m be_sa be_v be_la sz masz mvsz.
   (type_of_bir_exp be_m = SOME (BType_Mem masz mvsz)) ==>
   (type_of_bir_exp be_v = SOME (BType_Imm sz)) ==>
-  (symb_simplification_e sr
+  (birs_simplification_e
     (BExp_BinPred BIExp_Equal be_la be_sa)
     (BExp_Load
       (BExp_Store
@@ -118,11 +204,10 @@ val symb_simplification_Mem_Match_thm = store_thm(
 (* TODO: need one of these for 32bit stores as well, and the other two combinations *)
 val symb_simplification_Mem_Bypass_thm = store_thm(
    "symb_simplification_Mem_Bypass_thm", ``
-!sr.
 !be_m be_sa be_v be_la.
   (type_of_bir_exp be_m = SOME (BType_Mem Bit32 Bit8)) ==>
   (type_of_bir_exp be_v = SOME (BType_Imm Bit8)) ==>
-  (symb_simplification_e sr
+  (birs_simplification_e
     (BExp_BinExp BIExp_Or
        (BExp_BinPred BIExp_LessOrEqual
          (BExp_BinExp BIExp_Plus be_la (BExp_Const (Imm32 4w)))
